good progress on the encoding

experiments/LabelsInST.fst
@@ -12,13 +12,22 @@ type map_sharedT = mref (pos -> GTot bool) (fun (m0 m1:pos -> GTot bool) -> (for
 noeq
 type sigT = {
   map_shared : erased map_sharedT;
-  is_shared : #a:Type u#0 -> #p:preorder a -> r:mref a p -> h:heap -> res:Type0; //{next_addr h <= addr_of r ==> ~res};
-  share : #a:Type u#0 -> #p:preorder a -> sr:(mref a p) ->
+  is_shared : #a:Type0 -> #p:preorder a -> mref a p -> h:heap -> Type0;  // {h `contains` map_shared}
+  is_shared_stable : #a:Type0 -> r:ref a -> Lemma (stable (is_shared r)) [SMTPat (is_shared r)];
+  share : #a:Type0 -> #p:preorder a -> sr:(mref a p) ->
     ST unit 
-      (requires (fun h0 -> h0 `contains` sr))
+      (requires (fun h0 -> 
+        h0 `contains` sr /\
+        h0 `contains` map_shared /\
+        (addr_of sr =!= addr_of map_shared) /\ (** prevent sharing the map *)
+        ~(is_shared (map_shared) h0) /\
+        (forall p. p >= next_addr h0 ==> ~(sel h0 map_shared p)))) (** necessary to prove that freshly allocated references are not shared **)
       (ensures (fun h0 _ h1 ->
         modifies !{map_shared} h0 h1 /\
-        (forall b (r:ref b). h0 `contains` r /\ is_shared r h0 ==> is_shared r h1) /\
+        ~(is_shared (map_shared) h1) /\
+        (forall b (r:ref b). is_shared r h0 ==> is_shared r h1) /\
+        (forall b (r:ref b). ~(is_shared r h0) /\ addr_of r =!= addr_of sr ==> ~(is_shared r h1)) /\
+        (forall p. p >= next_addr h1 ==> ~(sel h1 map_shared p)) /\
         is_shared sr h1
 ))
 }
@@ -29,15 +38,38 @@ let secret_map : map_sharedT = (** In Pulse, this can be a ghost reference and `
 
 let shareS : sigT = {
   map_shared = secret_map;
-  //is_shared = (fun #a #p r h -> if addr_of r < next_addr h then (sel h secret_map) (addr_of r) else false);
-  is_shared = (fun #a #p r h -> (sel h secret_map) (addr_of r));
+  // is_shared = (fun #a #p r h -> addr_of r < next_addr h /\ (sel h secret_map) (addr_of r));
+  is_shared = (fun #a #p r h -> h `contains` secret_map /\ (** this contains is necessary to show that is_shared is a stable predicate **)
+                             (sel h secret_map) (addr_of r));
+  is_shared_stable = (fun #a r -> ());
   share = (fun #a #p sr -> 
+    let h0 = get () in
+    assume (addr_of sr < next_addr h0);(** Should be easy **)
     let m = !secret_map in
     let m' = (fun p -> if p = addr_of sr then true else m p) in
-    secret_map := m'
+    secret_map := m';
+    let h1 = get () in
+    assume (next_addr h0 <= next_addr h1)(** Should be easy **)
   );
 }
 
+  (**
+val is_shared_stable : #a:Type0 -> r:ref a -> Lemma (stable (shareS.is_shared r)) [SMTPat (shareS.is_shared r)]
+let is_shared_stable #a r : Lemma (stable (shareS.is_shared r)) [SMTPat (shareS.is_shared r)] = ()
+  (**assert (stable (shareS.is_shared r)) by (
+    norm[delta_only [`%stable;`%heap_rel];iota];
+    let h1 = forall_intro () in let h2 = forall_intro () in
+    let i = implies_intro () in 
+    let (x, y) = destruct_and i in
+    clear i;
+    let y = instantiate y (fresh_uvar None) in
+    let y' = instantiate y (fresh_uvar None) in
+    let y'' = instantiate y' (`secret_map) in
+    clear y; clear y';
+    compute ();
+    binder_retype (nth_binder 6); compute (); trefl ();
+    dump "H"
+  )**)**)
 
 unfold let unmodified_common (h0:heap) (h1:heap) : Type0 =
   (forall (a:Type) (rel:preorder a) (r:mref a rel).{:pattern (contains h1 r)}
@@ -53,8 +85,15 @@ let modifies_only_shared (h0:heap) (h1:heap) : Type0 =
 
 effect IST (a:Type) (pre:st_pre) (post: (h:heap -> Tot (st_post' a (pre h)))) =
   ST a 
-    (requires (fun h0      -> h0 `contains` shareS.map_shared /\ pre h0))
-    (ensures  (fun h0 r h1 -> post h0 r h1))
+    (requires (fun h0      -> 
+      h0 `contains` shareS.map_shared /\ 
+      ~(shareS.is_shared (shareS.map_shared) h0) /\ (* the map stays unshared *)
+      (forall p. p >= next_addr h0 ==> ~(sel h0 shareS.map_shared p)) /\
+      pre h0))
+    (ensures  (fun h0 r h1 -> 
+      ~(shareS.is_shared (shareS.map_shared) h1) /\
+      (forall p. p >= next_addr h1 ==> ~(sel h1 shareS.map_shared p)) /\
+      post h0 r h1))
 
 val progr_sep_test: 
   #rp: ref int -> 
@@ -71,7 +110,7 @@ let progr_sep_test #rp f =
 
 val progr_declassify :
   rp: ref int -> 
-  ctx:(r:(ref int) -> ST unit (fun h0 -> h0 `contains` r /\ shareS.is_shared r h0) (ensures (fun h0 _ h1 -> modifies_only_shared h0 h1))) ->
+  ctx:(r:(ref int) -> IST unit (fun h0 -> h0 `contains` r /\ shareS.is_shared r h0) (ensures (fun h0 _ h1 -> modifies_only_shared h0 h1))) ->
   IST unit
     (requires (fun h0 -> 
       h0 `contains` rp /\
@@ -83,7 +122,7 @@ let progr_declassify rp f =
 
 val progr_declassify_nested:
   rp: ref (ref int) -> 
-  ctx:(r:(ref (ref int)) -> ST unit 
+  ctx:(r:(ref (ref int)) -> IST unit 
     (requires (fun h0 -> h0 `contains` r /\ h0 `contains` (sel h0 r) /\ shareS.is_shared r h0 /\ shareS.is_shared (sel h0 r) h0))
     (ensures (fun h0 _ h1 -> modifies_only_shared h0 h1))) ->
   IST unit
@@ -100,7 +139,7 @@ let progr_declassify_nested rp f =
 val progr_secret_unchanged_test: 
   rp: ref int -> 
   rs: ref (ref int) ->
-  ctx:(unit -> ST unit (fun _ -> True) (fun h0 _ h1 -> modifies_only_shared h0 h1)) ->
+  ctx:(unit -> IST unit (fun _ -> True) (fun h0 _ h1 -> modifies_only_shared h0 h1)) ->
   IST unit 
     (requires (fun h0 -> 
       h0 `contains` rp /\ h0 `contains` rs /\ h0 `contains` (sel h0 rs) /\
@@ -113,59 +152,66 @@ val progr_secret_unchanged_test:
 let progr_secret_unchanged_test rp rs ctx = 
   let h0 = gst_get () in
   let secret: ref int = alloc 0 in
+  lemma_alloc (FStar.Heap.trivial_preorder int) h0 0 false;
+  assume (addr_of secret == next_addr h0); (** Should be easy **)
   let h1 = gst_get () in
-  assume (~(shareS.is_shared secret h1)); (** one needs to prove that a fresh reference is not shared **)
+  assume (next_addr h0 + 1 == next_addr h1);(** Should be easy **)
+  assert (~(shareS.is_shared secret h0)); 
+  assert (~(shareS.is_shared secret h1));
   ctx ();
   let v = !secret in
   assert (v == 0);
   ()
 
-(**
 val progr_passing_callback_test: 
   rp: ref int -> 
   rs: ref (ref int) ->
-  ctx:(elab_typ (TArr (TArr TUnit TUnit) TUnit)) ->
+  //ctx:(elab_typ (TArr (TArr TUnit TUnit) TUnit)) ->
+  ctx:( (unit -> IST unit (fun _ -> True) (fun h0 _ h1 -> modifies_only_shared h0 h1)) -> 
+              IST unit (fun _ -> True) (fun h0 _ h1 -> modifies_only_shared h0 h1)) ->
   IST unit 
     (requires (fun h0 ->
-      satisfy rp h0 contains_pred /\
-      label_of rp h0 == High /\
-      satisfy rs h0 is_low_pred))
+      h0 `contains` rp /\ h0 `contains` rs /\ h0 `contains` (sel h0 rs) /\
+      ~(shareS.is_shared rp h0) /\
+      shareS.is_shared rs h0 /\ shareS.is_shared (sel h0 rs) h0))
     (ensures (fun h0 _ h1 -> sel h0 rp == sel h1 rp)) // the content of rp should stay the same before/ after calling the context
 
 // TODO: the callback of the program should be able to modify rp
 let progr_passing_callback_test rp rs f =
-  let secret: ref int = ist_alloc #InvT_Nat 0 in
-  let h0 = get () in
-  declassify_low' #TNat secret;
-  let h1 = get () in
-  lemma_declassify_preserves_is_low InvT_Nat secret h0 h1;
-  mst_witness (contains_pred secret);
-  mst_witness (is_low_pred secret);
-  let cb: elab_typ (TArr TUnit TUnit) = (fun _ -> 
-    mst_recall (contains_pred secret);
-    mst_recall (is_low_pred secret);
-    elab_write #TNat secret (!secret + 1);
-    raise_val ()) in
-  downgrade_val (f cb);
-  ()
+  let h0 = gst_get () in
+  let secret: ref int = alloc 0 in
+  assume (addr_of secret == next_addr h0); (** Should be easy **)
+  let h1 = gst_get () in
+  assume (next_addr h0 <= next_addr h1);(** Should be easy **)
+  shareS.share secret;
+  gst_witness (contains_pred secret);
+  gst_witness (shareS.is_shared secret);
+  let cb : (unit -> IST unit (fun _ -> True) (fun h0 _ h1 -> modifies_only_shared h0 h1)) = (fun _ -> 
+    let h0 = gst_get () in
+    gst_recall (contains_pred secret);
+    gst_recall (shareS.is_shared secret);
+    secret := !secret + 1;
+    let h1 = gst_get () in
+    assume (next_addr h0 <= next_addr h1);
+    ()) in
+  f cb
 
 val progr_getting_callback_test: 
   rp: ref int -> 
   rs: ref (ref int) ->
-  ctx:(elab_typ (TArr TUnit (TArr TUnit TUnit))) ->
+  ctx:( unit -> 
+    IST ((unit -> IST unit (fun _ -> True) (fun h0 _ h1 -> modifies_only_shared h0 h1)))
+      (fun _ -> True)
+      (fun h0 _ h1 -> modifies_only_shared h0 h1)) ->
+ // ctx:(elab_typ (TArr TUnit (TArr TUnit TUnit))) ->
   IST unit 
     (requires (fun h0 ->
-      satisfy rp h0 contains_pred /\
-      label_of rp h0 == High /\
-      satisfy rs h0 is_low_pred))
+      h0 `contains` rp /\ h0 `contains` rs /\ h0 `contains` (sel h0 rs) /\
+      ~(shareS.is_shared rp h0) /\
+      shareS.is_shared rs h0 /\ shareS.is_shared (sel h0 rs) h0))
     (ensures (fun h0 _ h1 -> sel h0 rp == sel h1 rp))
+
 let progr_getting_callback_test rp rs f =
-  let h0 = get () in
-  let cb = f (raise_val ()) in
-  let h1 = get () in
-  downgrade_val (cb (raise_val ()));
-  let h2 = get () in
-  lemma_modifies_only_label_trans Low h0 h1 h2;
-  assert (modifies_only_label Low h0 h2);
+  let cb = f () in
+  cb ();
   ()
-**)
